theories/L6_PCPS/Heap/log_rel_post_cc.v
@@ -24,24 +24,348 @@ Module LogRelPostCC (H : Heap).
              (fR : fun_body_rel) : Prop :=
     match v1, v2 with
     | FunPtr B1 f1, FunPtr B2 f2 =>
-      forall H1' H1'' rho1 H2' b1 b2 ft1 xs1 e1 vs1 vs2,
-         Union_list (map val_loc vs1) |- H1 ≃_(id, b1) H1' ->
-         injective_subdomain (reach' H1' (Union_list (map val_loc vs1))) b1 ->
+      forall rho1 ft1 xs1 e1 vs1 vs2 b,        
+        find_def f1 B1 = Some (ft1, xs1, e1) ->
+        setlist xs1 vs1 (def_funs B1 B1 (M.empty _)) = Some rho1 ->
 
-         Union_list (map val_loc vs2) |- H2 ≃_(b2, id) H2' ->
-         injective_subdomain (reach' H2' (Union_list (map val_loc vs2))) b2 ->
-                                       
-         find_def f1 B1 = Some (ft1, xs1, e1) ->
-         setlist xs1 vs1 (def_funs B1 B1 (M.empty _)) = Some rho1 ->
-         live' (env_locs rho1 (occurs_free e1)) H1' H1'' b1 ->
-
-         length vs1 = length vs2 ->
-         
-         exists ft2 xs2 e2 rho2 H2'',
-           find_def f1 B1 = Some (ft2, xs2, e2) /\
-           setlist xs1 vs1 (def_funs B1 B1 (M.empty _)) = Some rho2 /\
-           live' (env_locs rho2 (occurs_free e2)) H2' H2'' b2 /\
-           fR GP GQ (b2 ∘ b ∘ b2) vs1 H1' vs2 H2' (H1'', rho1, e1) (H2'', rho2, e2)           
+        length vs1 = length vs2 ->
+        
+        exists ft2 xs2 e2 rho2,
+          find_def f1 B1 = Some (ft2, xs2, e2) /\
+          setlist xs1 vs1 (def_funs B1 B1 (M.empty _)) = Some rho2 /\
+          let GP' c1 c2 :=
+              let '(H1, rho1, c1) := c1 in
+              let '(H2, rho2, c2) := c2 in              
+              (forall H1' H2' b1 b2,
+                  live' (env_locs rho1 (occurs_free e1)) H1 H1' b1 ->
+                  live' (env_locs rho2 (occurs_free e2)) H2 H2' b2 ->
+                  GP (Empty_set _) _ 0 0 (H1', rho1, e1) (H2', rho2, e2)) in 
+          fR GP' (GP (Empty_set _) _ 0 0)
+             (GQ 0 0) b vs1 H1 vs2 H2 (H1, rho1, e1) (H2, rho2, e2)           
     | _, _ => False
-    end. 
+    end.
+
+  Definition no_clos_rel  (GP : GIInv) (GQ : GInv) (b : Inj)
+             (b1 : block) (H1 : heap block)
+             (b2 : block) (H2 : heap block)
+             (fR : fun_body_rel) (vR : val_rel) : Prop := False.
+
+  Instance Proper_clos_rel : forall P Q b b1 H1 b2 H2,
+      Proper ((pointwise_lifting iff fun_body_args) ==> (pointwise_lifting iff val_rel_args) ==> iff) (no_clos_rel P Q b b1 H1 b2 H2).
+  Proof. clear; now firstorder. Qed. 
+
+  Instance Proper_fun_rel : forall  P Q b v1 H1 v2 H2, Proper ((pointwise_lifting iff fun_body_args) ==> iff) (fun_ptr_rel P Q b v1 H1 v2 H2).
+  Proof.
+    intros. intros P1 P2 Hyp. split. 
+    - unfold fun_ptr_rel. destruct v1; destruct v2; eauto.
+      intros Hfun. intros.
+      edestruct Hfun as [ft2 [xs2 [e2 [rho2 [Hdef2 [Hset2 Hrel]]]]]]; try eassumption.
+      repeat eexists; eauto. eapply Hyp. eassumption.
+    - unfold fun_ptr_rel. destruct v1; destruct v2; eauto.
+      intros Hfun. intros.
+      edestruct Hfun as [ft2 [xs2 [e2 [rho2 [Hdef2 [Hset2 Hrel]]]]]]; try eassumption.
+      repeat eexists; eauto. eapply Hyp. eassumption.
+  Qed. 
       
+  Definition val_rel := val_log_rel big_step_GC_cc big_step_GC_cc no_clos_rel fun_ptr_rel. 
+  Definition exp_rel := exp_log_rel val_rel big_step_GC_cc big_step_GC_cc.
+  Definition var_rel := var_log_rel' big_step_GC_cc big_step_GC_cc no_clos_rel fun_ptr_rel.
+  Definition env_rel := env_log_rel_P' big_step_GC_cc big_step_GC_cc no_clos_rel fun_ptr_rel.
+  Definition heap_rel := heap_log_rel val_rel.
+
+  Definition val_rel' (k : nat)  (j : nat) (IP : GIInv) (P : GInv) (b : Inj) (r1 r2 : ans) : Prop :=
+    match r1, r2 with
+    | OOT, OOT => True (* Both programs timeout *)
+    | Res (v1, H1), Res (v2, H2) => (* Both programs terminate *)
+      match v1, v2 with
+      | Loc l1, Loc l2 =>
+        b l1 = l2 /\
+        match get l1 H1, get l2 H2 with
+        | Some (Constr c1 vs1), Some (Constr c2 vs2) =>
+          c1 = c2 /\ 
+          Forall2 (fun v1 v2 =>  forall i, (i < j)%nat -> val_rel k i IP P b (Res (v1, H1)) (Res (v2, H2))) vs1 vs2
+        | _, _ => False
+        end
+      | FunPtr B1 f1, FunPtr B2 f2 =>
+        forall rho1 ft1 xs1 e1 vs1 vs2 b,        
+          find_def f1 B1 = Some (ft1, xs1, e1) ->
+          setlist xs1 vs1 (def_funs B1 B1 (M.empty _)) = Some rho1 ->
+
+          length vs1 = length vs2 ->
+          
+          exists ft2 xs2 e2 rho2,
+            find_def f1 B1 = Some (ft2, xs2, e2) /\
+            setlist xs1 vs1 (def_funs B1 B1 (M.empty _)) = Some rho2 /\
+            forall i, (i < k)%nat ->
+                 (forall j, Forall2 (fun v1 v2 => val_rel i j IP P b (Res (v1, H1)) (Res (v2, H2))) vs1 vs2) ->
+                 (forall H1' H2' b1 b2,
+                     live' (env_locs rho1 (occurs_free e1)) H1 H1' b1 ->
+                     live' (env_locs rho2 (occurs_free e2)) H2 H2' b2 ->
+                     IP (Empty_set _) _ 0 0 (H1', rho1, e1) (H2', rho2, e2)) /\
+                 (forall j, exp_rel i j
+                               (IP (Empty_set _) _ 0 0) IP
+                               (P 0 0) P
+                               (H1, rho1, e1) (H2, rho2, e2))            
+      | _, _ => False
+      end
+    | _, _ => False
+    end.
+
+  Opaque val_log_rel val_log_rel'. 
+  
+  Lemma val_rel_eq k j IP P b r1 r2 :
+    val_rel k j IP P b r1 r2 <-> val_rel' k j IP P b r1 r2.
+  Proof.
+    destruct k; destruct j; 
+      destruct r1 as [[[l1 | lf1 f1] H1] |]; destruct r2 as [[[l2 | lf2 f2] H2] |];
+        try (now split; intros; contradiction);
+        try (now simpl; eauto).
+    simpl.
+    - split.
+      + simpl. intros [Hyp1 Hyp2]. split; eauto. 
+        destruct (get l1 H1) as [b1|]; destruct (get l2 H2) as [b2|]; try now eauto. 
+        destruct b1 as [c1 vs1 | v1 v2 | ]; try now eauto.
+        destruct b2 as [c2 vs2 | v1' v2' | ]; try contradiction.
+        destruct Hyp2 as [Hyp2 Hyp3]. split; eauto.
+        eapply Forall2_monotonic; [| eassumption ]. intros. omega.
+      + simpl. intros [Hyp1 Hyp2]. split; eauto. 
+        destruct (get l1 H1) as [b1|]; destruct (get l2 H2) as [b2|]; try now eauto. 
+        destruct b1 as [c1 vs1 | v1 v2 | ]; try now eauto.
+        destruct b2 as [c2 vs2 | v1' v2' | ]; try contradiction.
+        destruct Hyp2 as [Hyp2 Hyp3]. split; eauto.
+        eapply Forall2_monotonic; [| eassumption ]. intros. omega.
+    - simpl. split. 
+      intros Hyp. intros.
+      edestruct Hyp as [ft2 [xs2 [e2 [Hdef2 [Hset2 Hrel]]]]]; try eassumption.
+      do 4 eexists; repeat split; eauto. exfalso. omega. 
+      exfalso; omega.
+      
+      intros Hyp. intros.
+      edestruct Hyp as [ft2 [xs2 [e2 [Hdef2 [Hset2 Hrel]]]]]; try eassumption.
+      do 4 eexists; repeat split; eauto.
+
+    - split.
+      + simpl. intros [Hyp1 Hyp2]. split; eauto. 
+        destruct (get l1 H1) as [b1|]; destruct (get l2 H2) as [b2|]; try now eauto. 
+        destruct b1 as [c1 vs1 | v1 v2 | ]; try now eauto.
+        destruct b2 as [c2 vs2 | v1' v2' | ]; try contradiction.
+        destruct Hyp2 as [Hyp2 Hyp3]. split; eauto.
+        eapply Forall2_monotonic; [| eassumption ].
+        intros v1 v2 Hyp i Hlt. 
+        replace i with (j - (j - i)) by omega. eapply Hyp. omega.
+      + simpl. intros [Hyp1 Hyp2]. split; eauto. 
+        destruct (get l1 H1) as [b1|]; destruct (get l2 H2) as [b2|]; try now eauto. 
+        destruct b1 as [c1 vs1 | v1 v2 | ]; try now eauto.
+        destruct b2 as [c2 vs2 | v1' v2' | ]; try contradiction.
+        destruct Hyp2 as [Hyp2 Hyp3]. split; eauto.
+        eapply Forall2_monotonic; [| eassumption ].
+        intros v1 v2 Hyp i Hlt.
+        replace (j - (j - i)) with i by omega. eapply Hyp. omega.
+    - simpl. split. 
+      intros Hyp. intros.
+      edestruct Hyp as [ft2 [xs2 [e2 [Hdef2 [Hset2 Hrel]]]]]; try eassumption.
+      do 4 eexists; repeat split; eauto. exfalso. omega. 
+      exfalso; omega.
+      
+      intros Hyp. intros.
+      edestruct Hyp as [ft2 [xs2 [e2 [Hdef2 [Hset2 Hrel]]]]]; try eassumption.
+      do 4 eexists; repeat split; eauto.
+    - split.
+      + simpl. intros [Hyp1 Hyp2]. split; eauto. 
+        destruct (get l1 H1) as [b1|]; destruct (get l2 H2) as [b2|]; try now eauto. 
+        destruct b1 as [c1 vs1 | v1 v2 | ]; try now eauto.
+        destruct b2 as [c2 vs2 | v1' v2' | ]; try contradiction.
+        destruct Hyp2 as [Hyp2 Hyp3]. split; eauto.
+        eapply Forall2_monotonic; [| eassumption ]. intros. omega.
+      + simpl. intros [Hyp1 Hyp2]. split; eauto. 
+        destruct (get l1 H1) as [b1|]; destruct (get l2 H2) as [b2|]; try now eauto. 
+        destruct b1 as [c1 vs1 | v1 v2 | ]; try now eauto.
+        destruct b2 as [c2 vs2 | v1' v2' | ]; try contradiction.
+        destruct Hyp2 as [Hyp2 Hyp3]. split; eauto.
+        eapply Forall2_monotonic; [| eassumption ]. intros. omega.
+    - simpl. split. 
+      + intros Hyp. intros.  
+        edestruct Hyp as [ft2 [xs2 [rho2 [e2 [Hdef2 [Hset2 Hrel]]]]]]; try eassumption.
+        do 4 eexists; split; [| split ]; eauto. intros i Hlt Hall.
+        assert (Hieq : k - (k - i) = i) by omega. 
+        split.  
+        eapply Hrel; eauto. intros j.   
+        eapply Forall2_monotonic; [| now eapply (Hall j)  ].
+        intros v1 v2 Hyp'. rewrite Hieq. now eapply Hyp'.
+        
+        setoid_rewrite <- Hieq. eapply Hrel; eauto. intros j. 
+        eapply Forall2_monotonic; [| now eapply (Hall j)  ].
+        intros v1 v2 Hyp'. rewrite Hieq. eassumption.
+      + intros Hyp. intros. 
+        edestruct Hyp as [ft2 [xs2 [rho2 [e2 [Hdef2 [Hset2 Hrel]]]]]]; try eassumption.
+        do 4 eexists; split; [| split ]; eauto. intros i Hlt Hall.
+        assert (Hieq : k - (k - i) = i) by omega. 
+        split. 
+        eapply Hrel; eauto. intros j.  
+        eapply Forall2_monotonic; [| now eapply (Hall j)  ].
+        intros v1 v2 Hyp'. rewrite <- Hieq. now eapply Hyp'.
+        
+        setoid_rewrite  Hieq. eapply Hrel; eauto. intros j. 
+        eapply Forall2_monotonic; [| now eapply (Hall j)  ].
+        intros v1 v2 Hyp'. rewrite <- Hieq. eassumption.
+    - split.
+      + simpl. intros [Hyp1 Hyp2]. split; eauto. 
+        destruct (get l1 H1) as [b1|]; destruct (get l2 H2) as [b2|]; try now eauto. 
+        destruct b1 as [c1 vs1 | v1 v2 | ]; try now eauto.
+        destruct b2 as [c2 vs2 | v1' v2' | ]; try contradiction.
+        destruct Hyp2 as [Hyp2 Hyp3]. split; eauto.
+        eapply Forall2_monotonic; [| eassumption ].
+        intros v1 v2 Hyp i Hlt. 
+        replace i with (j - (j - i)) by omega. eapply Hyp. omega.
+      + simpl. intros [Hyp1 Hyp2]. split; eauto. 
+        destruct (get l1 H1) as [b1|]; destruct (get l2 H2) as [b2|]; try now eauto. 
+        destruct b1 as [c1 vs1 | v1 v2 | ]; try now eauto.
+        destruct b2 as [c2 vs2 | v1' v2' | ]; try contradiction.
+        destruct Hyp2 as [Hyp2 Hyp3]. split; eauto.
+        eapply Forall2_monotonic; [| eassumption ].
+        intros v1 v2 Hyp i Hlt.
+        replace (j - (j - i)) with i by omega. eapply Hyp. omega.
+    - simpl. split. 
+      + intros Hyp. intros. 
+        edestruct Hyp as [ft2 [xs2 [rho2 [e2 [Hdef2 [Hset2 Hrel]]]]]]; try eassumption.
+        do 4 eexists; split; [| split ]; eauto. intros i Hlt Hall.
+        assert (Hieq : k - (k - i) = i) by omega. 
+        split. 
+        eapply Hrel; eauto. intros j'.  
+        eapply Forall2_monotonic; [| now eapply (Hall j')  ].
+        intros v1 v2 Hyp'. rewrite Hieq. now eapply Hyp'. 
+        
+        setoid_rewrite <- Hieq. eapply Hrel; eauto. intros j'. 
+        eapply Forall2_monotonic; [| now eapply (Hall j')  ].
+        intros v1 v2 Hyp'. rewrite Hieq. eassumption.
+      + intros Hyp. intros. 
+        edestruct Hyp as [ft2 [xs2 [rho2 [e2 [Hdef2 [Hset2 Hrel]]]]]]; try eassumption.
+        do 4 eexists; split; [| split ]; eauto. intros i Hlt Hall.
+        assert (Hieq : k - (k - i) = i) by omega. 
+        split. 
+        eapply Hrel; eauto. intros j'.  
+        eapply Forall2_monotonic; [| now eapply (Hall j')  ].
+        intros v1 v2 Hyp'. rewrite <- Hieq. now eapply Hyp'. 
+        
+        setoid_rewrite  Hieq. eapply Hrel; eauto. intros j'. 
+        eapply Forall2_monotonic; [| now eapply (Hall j')  ].
+        intros v1 v2 Hyp'. rewrite <- Hieq. eassumption.
+
+        Grab Existential Variables. exact id. exact id.
+  Qed.
+
+  (** * Respects f_eq_subdomain *)
+
+  
+  Lemma val_rel_rename_ext IP P b b' k j r1 r2:
+    val_rel k j IP P b r1 r2 ->
+    f_eq_subdomain (reach_ans r1) b b' ->
+    val_rel k j IP P b' r1 r2.
+  Proof with (now eauto with Ensembles_DB).
+    rewrite !val_rel_eq in *. revert k j b b' r1 r2.
+    induction k as [k IHk] using lt_wf_rec1.
+    induction j as [j IHj] using lt_wf_rec1.
+    intros b b' [[v1 H1] | ] [[v2 H2] | ] Hres Hfeq; try contradiction; [| now eauto ].
+    destruct v1 as [l1 | lf1 f1]; destruct v2 as [l2 | lf2 f2]; simpl;
+    try contradiction; try (now simpl; eauto).
+    - simpl in Hres. destruct Hres as [Heq Hres]. 
+      destruct (get l1 H1) as [b1'|] eqn:Hget1; destruct (get l2 H2) as [b2'|] eqn:Hget2;
+        (try now eauto);
+        try (destruct b1' as [ | | ]; contradiction). 
+      split; eauto.
+      + rewrite <- Hfeq. eassumption.
+        eapply reach'_extensive. reflexivity.
+      + destruct b1' as [c1 vs1 | [? | B1 f1] [ env_loc1 |] | ]; try contradiction;
+          destruct b2' as [c2 vs2 | | ]; try contradiction. 
+        destruct Hres as [Hceq Hall]. split; eauto. 
+        eapply Forall2_monotonic_strong; [| eassumption ]. intros x1 x2 Hin1 Hin2 HR i Hlt.
+        rewrite val_rel_eq. eapply IHj. eassumption.
+        rewrite <- val_rel_eq. eapply HR; eauto.
+        
+        eapply f_eq_subdomain_antimon; [| eassumption ].
+        rewrite (reach_unfold H1 (val_loc (Loc l1))).
+        eapply Included_Union_preserv_r. eapply reach'_set_monotonic.
+        simpl. rewrite post_Singleton; [| eassumption ].
+        eapply In_Union_list. eapply in_map. eassumption.
+    (* - intros rho1 ft1 xs1 e1 vs1 vs2 Hdef1 Hset1 Hlen. *)
+    (*   edestruct Hres as [ft2 [xs2 [e2 [rho2 [Hdef2 [Hset2 Hrel]]]]]]; try eassumption. *)
+    (*   do 4 eexists. split. eassumption. split. eassumption. intros i Hlt Hall. *)
+    (*   eapply Hrel. eassumption. *)
+    (*   intros j'. *)
+      
+    (*   eapply Forall2_monotonic_strong; [| exact (Hall j') ]. intros x1 x2 Hin1 Hin2 HR. *)
+    (*   rewrite val_rel_eq. eapply IHk. eassumption. *)
+    (*   rewrite <- val_rel_eq. eapply HR; eauto. *)
+    (*   symmetry.  *)
+    (*   eapply f_eq_subdomain_antimon; [| eassumption ]. *)
+    (*   rewrite (reach_unfold H1 (val_loc (Loc l1))). *)
+    (*   eapply Included_Union_preserv_r. eapply reach'_set_monotonic. *)
+    (*   simpl. rewrite post_Singleton; [| eassumption ]. *)
+    (*   eapply In_Union_list. eapply in_map. eassumption. *)
+      
+    (*   ; eauto. exfalso. omega.  *)
+    (*   exfalso; omega. *)
+      
+    (*   intros Hyp. intros. *)
+    (*   edestruct Hyp as [ft2 [xs2 [e2 [Hdef2 [Hset2 Hrel]]]]]; try eassumption. *)
+    (*   do 4 eexists; repeat split; eauto. *)
+  Qed.
+
+  Lemma var_rel_rename_ext k j IP P b b' H1 H2 rho1 rho2 x y: 
+    var_rel k j IP P b H1 rho1 H2 rho2 x y ->
+    f_eq_subdomain (reach' H1 (env_locs rho1 [set x])) b b' ->
+    var_rel k j IP P b' H1 rho1 H2 rho2 x y.
+  Proof with (now eauto with Ensembles_DB).
+    intros Hcc Heq v Hget. edestruct Hcc as [l2 [Hget2 Hres]].
+    eassumption. eexists; split; eauto.
+    rewrite <- val_log_rel_eq in *; tci.
+    eapply val_rel_rename_ext. eassumption.
+    eapply f_eq_subdomain_antimon; [| eassumption ].
+    eapply reach'_set_monotonic. eapply env_locs_Singleton; try eassumption.
+  Qed. 
+  
+  Lemma env_rel_rename_ext S k j IP P b b' H1 H2 rho1 rho2 : 
+    env_rel S k j IP P b (H1, rho1) (H2, rho2) ->
+    f_eq_subdomain (reach' H1 (env_locs rho1 S)) b b' ->
+    env_rel S k j IP P b' (H1, rho1) (H2, rho2).
+  Proof with (now eauto with Ensembles_DB).
+    intros Henv Heq x Hin v Hget. 
+    eapply var_rel_rename_ext. eapply Henv. 
+    eassumption. eapply f_eq_subdomain_antimon; [| eassumption ].
+    eapply reach'_set_monotonic. eapply env_locs_monotonic.
+    eapply Singleton_Included. eassumption.
+    eassumption.
+  Qed.
+
+
+  Lemma heap_rel_rename_ext S k j IP P b b' H1 H2 : 
+    heap_rel S k j IP P b H1 H2 ->
+    f_eq_subdomain (reach' H1 S) b b' ->
+    heap_rel S k j IP P b' H1 H2.
+  Proof with (now eauto with Ensembles_DB).
+    intros Hheap Hfeq x Hin.
+    eapply val_rel_rename_ext. 
+    rewrite <- Hfeq. eapply Hheap. eassumption.
+    eapply reach'_extensive. eassumption.
+    eapply f_eq_subdomain_antimon; [| eassumption ].
+    eapply reach'_set_monotonic.
+    eapply Singleton_Included. eassumption.
+  Qed.
+
+
+  
+
+    
+  (** * Logical relation respects heap_equivalence *)  
+  
+  (** * Well-formedness/closedness lemmas *)
+
+  (** * Heap monotonicity/allocation  *)
+  
+  (** * Reachable locations image *)
+
+  (** * Compatibility lemmas *)
+
+End LogRelPostCC. 
+
+  
